sha/XorCorrespondence.v
@@ -3,177 +3,119 @@ Require Import compcert.lib.Integers.
 Require Import compcert.lib.Coqlib.
 Require Import List.
 Require Import List. Import ListNotations.
+Require Import sha.hmac_pure_lemmas.
 
 Definition asZ (x : bool) : Z := if x then 1 else 0.
 
 Lemma asZT: asZ true = 1. reflexivity. Qed.
 Lemma asZF: asZ false = 0. reflexivity. Qed.
 
-Definition convertByteBits bits (byte : Z) : Prop :=
+Definition convertByteBits bits (b : byte) : Prop :=
   exists (b0 b1 b2 b3 b4 b5 b6 b7 : bool),
    bits = [b0; b1; b2; b3; b4; b5; b6; b7] /\
-   byte =  (1 * (asZ b0) + 2 * (asZ b1) + 4 * (asZ b2) + 8 * (asZ b3)
+   Byte.unsigned b =  (1 * (asZ b0) + 2 * (asZ b1) + 4 * (asZ b2) + 8 * (asZ b3)
          + 16 * (asZ b4) + 32 * (asZ b5) + 64 * (asZ b6) + 128 * (asZ b7)).
-(* TODO: stuck here *)
 
-Lemma AUX1 b2 b3 b4 b5 b6 b7 b8 b9 b10 b11 b12 b13 b14 b15:
-Z.lxor
-  (1 * 1 + 2 * 1 + 4 * asZ b2 + 8 * asZ b3 + 16 * asZ b4 + 32 * asZ b5 +
-   64 * asZ b6 + 128 * asZ b7)
-  (1 * asZ b8 + 2 * asZ b9 + 4 * asZ b10 + 8 * asZ b11 + 16 * asZ b12 +
-   32 * asZ b13 + 64 * asZ b14 + 128 * asZ b15) =
-1 * (if negb b8 then 1 else 0) + 2 * (if negb b9 then 1 else 0) +
-4 * (if xorb b2 b10 then 1 else 0) + 8 * (if xorb b3 b11 then 1 else 0) +
-16 * (if xorb b4 b12 then 1 else 0) + 32 * (if xorb b5 b13 then 1 else 0) +
-64 * (if xorb b6 b14 then 1 else 0) + 128 * (if xorb b7 b15 then 1 else 0).
+Lemma testbit_b2z_nonzero:
+  forall i, i<>0 -> forall b, Z.testbit (Z.b2z b) i = false.
 Proof.
-      destruct b2; try rewrite asZT; try rewrite asZF.
-      { rewrite (xorb_true_l b10).
-        destruct b3; try rewrite asZT; try rewrite asZF.
-        { rewrite (xorb_true_l b11).
-          destruct b4; destruct b5; destruct b6; destruct b7; destruct b8; destruct b9;
-          destruct b10; destruct b11; destruct b12; destruct b13; destruct b14; destruct b15; trivial.
-        }
-        { rewrite (xorb_false_l b11).
-          destruct b4; destruct b5; destruct b6; destruct b7; destruct b8; destruct b9;
-          destruct b10; destruct b11; destruct b12; destruct b13; destruct b14; destruct b15; trivial.
-        }
-      }
-      { rewrite (xorb_false_l b10).
-        destruct b3; try rewrite asZT; try rewrite asZF.
-        { rewrite (xorb_true_l b11).
-          destruct b4; destruct b5; destruct b6; destruct b7; destruct b8; destruct b9;
-          destruct b10; destruct b11; destruct b12; destruct b13; destruct b14; destruct b15; trivial.
-        }
-        { rewrite (xorb_false_l b11).
-          destruct b4; destruct b5; destruct b6; destruct b7; destruct b8; destruct b9;
-          destruct b10; destruct b11; destruct b12; destruct b13; destruct b14; destruct b15; trivial.
-        }
-      }
-Qed.
-Lemma AUX2 b2 b3 b4 b5 b6 b7 b8 b9 b10 b11 b12 b13 b14 b15:
-Z.lxor (1 * 1 + 2 * 0 + 4 * asZ b2 + 8 * asZ b3 + 16 * asZ b4 + 32 * asZ b5 +
-   64 * asZ b6 + 128 * asZ b7)
-  (1 * asZ b8 + 2 * asZ b9 + 4 * asZ b10 + 8 * asZ b11 + 16 * asZ b12 +
-   32 * asZ b13 + 64 * asZ b14 + 128 * asZ b15) =
-1 * (if negb b8 then 1 else 0) + 2 * (if b9 then 1 else 0) +
-4 * (if xorb b2 b10 then 1 else 0) + 8 * (if xorb b3 b11 then 1 else 0) +
-16 * (if xorb b4 b12 then 1 else 0) + 32 * (if xorb b5 b13 then 1 else 0) +
-64 * (if xorb b6 b14 then 1 else 0) + 128 * (if xorb b7 b15 then 1 else 0).
-Proof.
-      destruct b2; try rewrite asZT; try rewrite asZF.
-      { rewrite (xorb_true_l b10).
-        destruct b3; try rewrite asZT; try rewrite asZF.
-        { rewrite (xorb_true_l b11).
-          destruct b4; destruct b5; destruct b6; destruct b7; destruct b8; destruct b9;
-          destruct b10; destruct b11; destruct b12; destruct b13; destruct b14; destruct b15; trivial.
-        }
-        { rewrite (xorb_false_l b11).
-          destruct b4; destruct b5; destruct b6; destruct b7; destruct b8; destruct b9;
-          destruct b10; destruct b11; destruct b12; destruct b13; destruct b14; destruct b15; trivial.
-        }
-      }
-      { rewrite (xorb_false_l b10).
-        destruct b3; try rewrite asZT; try rewrite asZF.
-        { rewrite (xorb_true_l b11).
-          destruct b4; destruct b5; destruct b6; destruct b7; destruct b8; destruct b9;
-          destruct b10; destruct b11; destruct b12; destruct b13; destruct b14; destruct b15; trivial.
-        }
-        { rewrite (xorb_false_l b11).
-          destruct b4; destruct b5; destruct b6; destruct b7; destruct b8; destruct b9;
-          destruct b10; destruct b11; destruct b12; destruct b13; destruct b14; destruct b15; trivial.
-        }
-      }
+intros.
+unfold Z.testbit, Z.b2z.
+destruct i; try contradiction; auto.
+destruct b; simpl; auto.
 Qed.
 
-Lemma AUX3 b2 b3 b4 b5 b6 b7 b8 b9 b10 b11 b12 b13 b14 b15:
-Z.lxor
-  (1 * 0 + 2 * 1 + 4 * asZ b2 + 8 * asZ b3 + 16 * asZ b4 + 32 * asZ b5 +
-   64 * asZ b6 + 128 * asZ b7)
-  (1 * asZ b8 + 2 * asZ b9 + 4 * asZ b10 + 8 * asZ b11 + 16 * asZ b12 +
-   32 * asZ b13 + 64 * asZ b14 + 128 * asZ b15) =
-1 * (if b8 then 1 else 0) + 2 * (if negb b9 then 1 else 0) +
-4 * (if xorb b2 b10 then 1 else 0) + 8 * (if xorb b3 b11 then 1 else 0) +
-16 * (if xorb b4 b12 then 1 else 0) + 32 * (if xorb b5 b13 then 1 else 0) +
-64 * (if xorb b6 b14 then 1 else 0) + 128 * (if xorb b7 b15 then 1 else 0).
+Lemma testbit_shiftl_8:
+  forall a0 a1 a2 a3 a4 a5 a6 a7,
+ forall i,
+  Z.testbit (Z.shiftl (Z.b2z a0) 0 + Z.shiftl (Z.b2z a1) 1
+             + Z.shiftl (Z.b2z a2) 2 + Z.shiftl (Z.b2z a3) 3
+             + Z.shiftl (Z.b2z a4) 4 + Z.shiftl (Z.b2z a5) 5
+             + Z.shiftl (Z.b2z a6) 6 + Z.shiftl (Z.b2z a7) 7)  i=
+   Z.testbit (Z.shiftl (Z.b2z a0) 0) i ||
+   Z.testbit (Z.shiftl (Z.b2z a1) 1) i ||
+   Z.testbit (Z.shiftl (Z.b2z a2) 2) i ||
+   Z.testbit (Z.shiftl (Z.b2z a3) 3) i ||
+   Z.testbit (Z.shiftl (Z.b2z a4) 4) i ||
+   Z.testbit (Z.shiftl (Z.b2z a5) 5) i ||
+   Z.testbit (Z.shiftl (Z.b2z a6) 6) i ||
+   Z.testbit (Z.shiftl (Z.b2z a7) 7) i.
 Proof.
-      destruct b2; try rewrite asZT; try rewrite asZF.
-      { rewrite (xorb_true_l b10).
-        destruct b3; try rewrite asZT; try rewrite asZF.
-        { rewrite (xorb_true_l b11).
-          destruct b4; destruct b5; destruct b6; destruct b7; destruct b8; destruct b9;
-          destruct b10; destruct b11; destruct b12; destruct b13; destruct b14; destruct b15; trivial.
-        }
-        { rewrite (xorb_false_l b11).
-          destruct b4; destruct b5; destruct b6; destruct b7; destruct b8; destruct b9;
-          destruct b10; destruct b11; destruct b12; destruct b13; destruct b14; destruct b15; trivial.
-        }
-      }
-      { rewrite (xorb_false_l b10).
-        destruct b3; try rewrite asZT; try rewrite asZF.
-        { rewrite (xorb_true_l b11).
-          destruct b4; destruct b5; destruct b6; destruct b7; destruct b8; destruct b9;
-          destruct b10; destruct b11; destruct b12; destruct b13; destruct b14; destruct b15; trivial.
-        }
-        { rewrite (xorb_false_l b11).
-          destruct b4; destruct b5; destruct b6; destruct b7; destruct b8; destruct b9;
-          destruct b10; destruct b11; destruct b12; destruct b13; destruct b14; destruct b15; trivial.
-        }
-      }
-Qed.
+intros.
+      destruct (zlt i 0).
+       rewrite !Z.testbit_neg_r by auto. reflexivity.
+       assert (0 <= i) by omega. clear g.
+     rewrite ?Z.shiftl_spec by auto.
+repeat rewrite <- Z.add_assoc.
+rewrite !Z.shiftl_mul_pow2 by omega.
+rewrite ?(Z.mul_comm (Z.b2z _)).
+unfold Z.pow, Z.pow_pos, Pos.iter.
+rewrite <- ?Z.mul_assoc.
+rewrite <- ?Z.mul_add_distr_l.
+rewrite ?Z.mul_1_l.
+rewrite ?(Z.add_comm _ (2 * _)).
+destruct (zlt i 1). {
+assert (i=0) by omega; subst i; clear H l; simpl Z.sub.
+rewrite ?Z.b2z_bit0.
+rewrite !testbit_b2z_nonzero by omega; rewrite ?orb_false_r.
+rewrite ?Z.add_bit0.
+rewrite ?Z.b2z_bit0.
+rewrite Z.testbit_even_0. rewrite xorb_false_l. reflexivity.
+}
+clear H.
+do 7
+match goal with H: i >= ?a |- _ =>
+let i' := constr:(Z.succ a) in let i' := eval compute in i' in 
+ let H' := fresh "H" in 
+destruct (zlt i i'); 
+  [assert (H': i=a) by omega;
+      change a with (Recdef.iter _ (Z.to_nat a) Z.succ 0) in H';
+      simpl Z.to_nat in H'; unfold Recdef.iter in H';
+      subst i; clear H;
+   rewrite Z.testbit_succ_r by omega;
+   rewrite ?Z.b2z_bit0;
+   rewrite !testbit_b2z_nonzero by omega; 
+   rewrite ?orb_false_r, ?orb_false_l;
+   rewrite ?Z.testbit_succ_r by omega;
+   rewrite ?Z.add_bit0;
+   rewrite ?Z.testbit_even_0;
+   rewrite ?Z.b2z_bit0;
+   rewrite ?orb_false_l;
+   rewrite ?xorb_false_l;
+   auto
+    | clear H]
+end.
 
-Lemma AUX4 b2 b3 b4 b5 b6 b7 b8 b9 b10 b11 b12 b13 b14 b15:
-Z.lxor (1 * 0 + 2 * 0 + 4 * asZ b2 + 8 * asZ b3 + 16 * asZ b4 + 32 * asZ b5 +
-   64 * asZ b6 + 128 * asZ b7)
-  (1 * asZ b8 + 2 * asZ b9 + 4 * asZ b10 + 8 * asZ b11 + 16 * asZ b12 +
-   32 * asZ b13 + 64 * asZ b14 + 128 * asZ b15) =
-1 * (if b8 then 1 else 0) + 2 * (if b9 then 1 else 0) +
-4 * (if xorb b2 b10 then 1 else 0) + 8 * (if xorb b3 b11 then 1 else 0) +
-16 * (if xorb b4 b12 then 1 else 0) + 32 * (if xorb b5 b13 then 1 else 0) +
-64 * (if xorb b6 b14 then 1 else 0) + 128 * (if xorb b7 b15 then 1 else 0).
-Proof.
-      destruct b2; try rewrite asZT; try rewrite asZF.
-      { rewrite (xorb_true_l b10).
-        destruct b3; try rewrite asZT; try rewrite asZF.
-        { rewrite (xorb_true_l b11).
-          destruct b4; destruct b5; destruct b6; destruct b7; destruct b8; destruct b9;
-          destruct b10; destruct b11; destruct b12; destruct b13; destruct b14; destruct b15; trivial.
-        }
-        { rewrite (xorb_false_l b11).
-          destruct b4; destruct b5; destruct b6; destruct b7; destruct b8; destruct b9;
-          destruct b10; destruct b11; destruct b12; destruct b13; destruct b14; destruct b15; trivial.
-        }
-      }
-      { rewrite (xorb_false_l b10).
-        destruct b3; try rewrite asZT; try rewrite asZF.
-        { rewrite (xorb_true_l b11).
-          destruct b4; destruct b5; destruct b6; destruct b7; destruct b8; destruct b9;
-          destruct b10; destruct b11; destruct b12; destruct b13; destruct b14; destruct b15; trivial.
-        }
-        { rewrite (xorb_false_l b11).
-          destruct b4; destruct b5; destruct b6; destruct b7; destruct b8; destruct b9;
-          destruct b10; destruct b11; destruct b12; destruct b13; destruct b14; destruct b15; trivial.
-        }
-      }
+rewrite !testbit_b2z_nonzero by omega; rewrite ?orb_false_r, ?orb_false_l.
+do 7 match goal with |- Z.testbit _ ?a = false =>
+  replace a with (Z.succ (Z.pred a)) by (clear; omega);
+  rewrite Z.testbit_succ_r by omega
+end.
+rewrite testbit_b2z_nonzero by omega.
+auto.
 Qed.
 
 Lemma xor_correspondence :
   forall (b0 b1 b2 b3 b4 b5 b6 b7 b8 b9 b10 b11 b12 b13 b14 b15 : bool)
-         (byte0 byte1 : Z),
+         (byte0 byte1 : byte),
     convertByteBits [b0; b1; b2; b3; b4; b5; b6; b7] byte0 ->
     convertByteBits [b8; b9; b10; b11; b12; b13; b14; b15] byte1 ->
 
     convertByteBits
       [xorb b0 b8; xorb b1 b9; xorb b2 b10; xorb b3 b11;
        xorb b4 b12; xorb b5 b13; xorb b6 b14; xorb b7 b15]
-      (Z.lxor byte0 byte1).
+      (Byte.xor byte0 byte1).
 Proof.
   intros.
   generalize dependent H. generalize dependent H0. intros H0 H1.
   unfold convertByteBits. unfold asZ.
-
+  unfold Byte.xor.
+  rewrite Byte.unsigned_repr.
+*
   do 8 eexists. split. reflexivity.
   unfold convertByteBits in *.
+  set (a0 := Byte.unsigned byte0) in *. clearbody a0.
+  set (a1 := Byte.unsigned byte1) in *. clearbody a1.
 
   destruct H0 as [ ? [ ? [ ? [ ? [ ? [ ? [ ? [ ? ? ] ] ] ]] ]] ].  (* nested 8 *)
   destruct H.
@@ -186,15 +128,45 @@ Proof.
   symmetry in H.
   inversion H. clear H.
   subst.
-  destruct b0; try rewrite asZT; try rewrite asZF.
-  { rewrite (xorb_true_l b8).
-    destruct b1; try rewrite asZT; try rewrite asZF.
-    { rewrite (xorb_true_l b9). apply AUX1. }
-    { rewrite (xorb_false_l b9). apply AUX2. }
-  }
-  { rewrite (xorb_false_l b8).
-    destruct b1; try rewrite asZT; try rewrite asZF.
-    { rewrite (xorb_true_l b9). apply AUX3. }
-    { rewrite (xorb_false_l b9). apply AUX4. }
-  }
+      fold (asZ (xorb b2 b10)).
+      fold (asZ (xorb b4 b12)).
+      fold (asZ (xorb b6 b14)).
+      fold (asZ (xorb b0 b8)).
+      fold (asZ (xorb b1 b9)).
+      fold (asZ (xorb b3 b11)).
+      fold (asZ (xorb b5 b13)).
+      fold (asZ (xorb b7 b15)).
+      rewrite <- !(Z.mul_comm (asZ _)).
+      rewrite <- !(Z.shiftl_mul_pow2 _ 0) by (clear; omega).
+      rewrite <- !(Z.shiftl_mul_pow2 _ 1) by (clear; omega).
+      rewrite <- !(Z.shiftl_mul_pow2 _ 2) by (clear; omega).
+      rewrite <- !(Z.shiftl_mul_pow2 _ 3) by (clear; omega).
+      rewrite <- !(Z.shiftl_mul_pow2 _ 4) by (clear; omega).
+      rewrite <- !(Z.shiftl_mul_pow2 _ 5) by (clear; omega).
+      rewrite <- !(Z.shiftl_mul_pow2 _ 6) by (clear; omega).
+      rewrite <- !(Z.shiftl_mul_pow2 _ 7) by (clear; omega).
+      apply Z.bits_inj.
+      intro i.
+      rewrite Z.lxor_spec.
+      change asZ with Z.b2z.
+      destruct (zlt i 0).
+       rewrite !Z.testbit_neg_r by auto. reflexivity.
+       assert (0 <= i) by omega. clear g.
+
+       rewrite !testbit_shiftl_8.
+       rewrite !Z.shiftl_spec by auto.
+       destruct (zlt i 8).
+       2:{  rewrite !testbit_b2z_nonzero by omega; reflexivity. }
+       assert (i=0 \/ i=1 \/ i=2 \/ i=3 \/ i=4 \/ i=5 \/ i=6 \/ i=7) by omega.
+       decompose [or] H0; subst i; clear;
+       simpl Z.sub; rewrite ?orb_false_r;
+       rewrite ?Z.b2z_bit0;
+       rewrite ?testbit_b2z_nonzero by omega; simpl; auto.
+*
+      rewrite xor_inrange.
+      all: change Byte.modulus with 256 in *.
+      pose proof (Z_mod_lt (Z.lxor (Byte.unsigned byte0) (Byte.unsigned byte1)) 256).
+      assert (256>0) by omega. specialize (H H2).
+      change Byte.max_unsigned with 255. omega.
+      all: symmetry; apply Z.mod_small; apply Byte.unsigned_range.
 Qed.
