sha/hmac_common_lemmas.v
@@ -12,18 +12,9 @@ Require Import sha.spec_sha.
 
 Require Import sha.HMAC_functional_prog.
 Require Import sha.HMAC256_functional_prog.
-(*
-Lemma SF_ByteRepr x: isbyteZ x ->
-                     HP.HMAC_SHA256.sixtyfour x =
-                     map Byte.unsigned (HP.HMAC_SHA256.sixtyfour (Byte.repr x)).
-Proof. intros. unfold HP.HMAC_SHA256.sixtyfour.
- rewrite map_list_repeat.
- rewrite Byte.unsigned_repr; trivial. destruct H.
- assert (BMU: Byte.max_unsigned = 255). reflexivity. omega.
-Qed.
-*)
-Lemma str_to_Z_length: forall k,
-      String.length k = length (str_to_Z k).
+
+Lemma str_to_bytes_length: forall k,
+      String.length k = length (str_to_bytes k).
 Proof. intros. induction k; simpl; auto. Qed.
 
 Lemma first64_sixtyfour {A} (a:A):
@@ -36,19 +27,11 @@ Proof.
   rewrite length_list_repeat; trivial.
 Qed.
 
-Lemma Zlength_mkArgZ k pad: Zlength (HMAC_SHA256.mkArgZ k pad) = Z.of_nat (min (length k) 64).
+Lemma Zlength_mkArgZ k pad: Zlength (HMAC_SHA256.mkArg k pad) = Z.of_nat (min (length k) 64).
 Proof. intros. repeat rewrite Zlength_correct.
-   unfold HMAC_SHA256.mkArgZ, HMAC_SHA256.mkArg, HMAC_SHA256.sixtyfour.
+   unfold HMAC_SHA256.mkArg, HMAC_SHA256.sixtyfour.
    repeat rewrite map_length.
    rewrite combine_length, length_list_repeat . trivial.
-Qed.
-
-Lemma zeropad_isbyteZ: forall l, Forall isbyteZ l -> Forall isbyteZ (HMAC_SHA256.zeroPad l).
-Proof. unfold isbyteZ, HMAC_SHA256.zeroPad; intros.
-  rewrite Forall_forall in *. intros.
-  apply in_app_or in H0.
-  destruct H0. apply (H _ H0).
-  apply in_list_repeat in H0. (*apply In_Nlist in H0.*) subst; omega.
 Qed.
 
 Lemma nth_zeropad_left {d d'}: forall l i (I: 0<= i < Zlength l),
@@ -70,7 +53,7 @@ Proof.
 Qed.
 
 Lemma nth_zeropad_right {d} l i (I: Zlength l <= i < 64):
-      nth (Z.to_nat i) (HMAC_SHA256.zeroPad l) d = Z0.
+      nth (Z.to_nat i) (HMAC_SHA256.zeroPad l) d = Byte.zero.
 Proof. unfold HMAC_SHA256.zeroPad.
   specialize (Zlength_nonneg l). intros.
   rewrite app_nth2. rewrite nth_list_repeat'. trivial.
@@ -87,7 +70,7 @@ Qed.
 
 Lemma mkKey_right {d}: forall l (L: false = (Zlength l >? 64))
         i (I: Zlength l <= i < 64),
-      nth (Z.to_nat i) (HMAC_SHA256.mkKey l) d = Z0.
+      nth (Z.to_nat i) (HMAC_SHA256.mkKey l) d = Byte.zero.
 Proof.
   unfold HMAC_SHA256.mkKey. intros. simpl. rewrite <- L.
   apply nth_zeropad_right; trivial.
@@ -101,7 +84,7 @@ Qed.
 Lemma length_SHA256': forall l,
   length (functional_prog.SHA_256' l) = SHA256.DigestLength.
 Proof. intros. unfold functional_prog.SHA_256'. simpl.
-  rewrite length_intlist_to_Zlist, functional_prog.length_process_msg. reflexivity.
+  rewrite length_intlist_to_bytelist, functional_prog.length_process_msg. reflexivity.
 Qed.
 
 Lemma mkKey_length l: length (HMAC_SHA256.mkKey l) = SHA256.BlockSize.
@@ -123,36 +106,6 @@ Proof. unfold HMAC_SHA256.mkKey. rewrite Zlength_correct.
   simpl. unfold HMAC_SHA256.zeroPad. rewrite H. simpl.
   apply app_nil_r.
 Qed.
-
-Lemma isbyteZ_mkKey: forall l, Forall isbyteZ l -> Forall isbyteZ (HMAC_SHA256.mkKey l).
-Proof. intros.
-  unfold HMAC_SHA256.mkKey.
-  remember (Zlength l >? Z.of_nat SHA256.BlockSize).
-  destruct b.
-    apply zeropad_isbyteZ. apply SHA256.Hash_isbyteZ.
-    apply zeropad_isbyteZ; trivial.
-Qed.
-
-Lemma isbyte_hmac ipad opad m k:
-   Forall isbyteZ (HMAC_SHA256.HMAC ipad opad m k).
-Proof. apply SHA256.Hash_isbyteZ.  Qed.
-(*
-Lemma updAbs_len: forall L s t, update_abs L s t -> s256a_len t = s256a_len s + Zlength L * 8.
-Proof. intros. inversion H; clear H.
-  unfold s256a_len, bitlength. simpl.
-  rewrite Zlength_app. subst.
-  repeat rewrite Z.mul_add_distr_r.
-  repeat rewrite <- Z.add_assoc.
-  assert (Zlength blocks * WORD * 8 + Zlength newfrag * 8 =
-          Zlength oldfrag * 8 + Zlength L * 8).
-    assert (Zlength (oldfrag ++ L) = Zlength (intlist_to_Zlist blocks ++ newfrag)).
-      rewrite H4; trivial.
-    clear H4. rewrite Zlength_app in H.
-              rewrite <- (Z.mul_add_distr_r (Zlength oldfrag)), H. clear H.
-              rewrite Zlength_app, Zlength_intlist_to_Zlist.
-(*              rewrite (Z.mul_comm WORD). *) rewrite Z.mul_add_distr_r. trivial.
-  rewrite H; trivial.
-Qed.*)
 
 Lemma HMAC_length d k: length (HMAC256 d k) = 32%nat.
 Proof.
